src/cose/rust/CommonPulse.fst
@@ -1,0 +1,769 @@
+module CommonPulse
+#lang-pulse
+open Pulse
+open COSE.Format
+open Pulse.Lib.Trade
+open Pulse.Lib.Trade.Util
+open EverCrypt.Ed25519
+// module AP = Pulse.Lib.ArrayPtr
+module S = Pulse.Lib.Slice
+module V = Pulse.Lib.Vec
+module A = Pulse.Lib.Array
+open CDDL.Pulse.Types
+
+[@@pulse_unfold]
+let borrows (what from: slprop) : slprop =
+  what ** trade what from
+
+let specnint_of_int (i: int { - pow2 64 <= i /\ i < 0 }) : GTot spect_evercddl_nint_pretty =
+  Mkspect_evercddl_nint_pretty0 (UInt64.uint_to_t (-i-1))
+
+let specuint_of_int (i: int { 0 <= i /\ i < pow2 64 }) : GTot spect_evercddl_uint_pretty =
+  Mkspect_evercddl_uint_pretty0 (UInt64.uint_to_t i)
+
+let specint_of_int (i: int { -pow2 64 <= i /\ i < pow2 64 }) : GTot spect_evercddl_int_pretty =
+  if i >= 0 then
+    Mkspect_evercddl_int_pretty0 (specuint_of_int i)
+  else
+    Mkspect_evercddl_int_pretty1 (specnint_of_int i)
+
+inline_for_extraction noextract
+let i32_to_u64_safe (i: Int32.t { Int32.v i >= 0 }) : j:UInt64.t { UInt64.v j == Int32.v i } =
+  Math.Lemmas.pow2_lt_compat 64 31;
+  Math.Lemmas.small_mod (Int32.v i) (pow2 64);
+  Int.Cast.int32_to_uint64 i
+
+let specint_of_i32 (i: Int32.t) : GTot spect_evercddl_int_pretty =
+  Math.Lemmas.pow2_lt_compat 64 31;
+  specint_of_int (Int32.v i)
+
+let rel_evercddl_uint_eq a b : squash (rel_evercddl_uint a b == pure (Mkevercddl_uint_pretty0?._x0 a == Mkspect_evercddl_uint_pretty0?._x0 b)) = ()
+let rel_evercddl_nint_eq a b : squash (rel_evercddl_nint a b == pure (Mkevercddl_nint_pretty0?._x0 a == Mkspect_evercddl_nint_pretty0?._x0 b)) = ()
+
+let rel_evercddl_int_eq a b : squash (rel_evercddl_int a b ==
+  (match a, b with
+   | Mkevercddl_int_pretty0 a, Mkspect_evercddl_int_pretty0 b -> rel_evercddl_uint a b
+   | Mkevercddl_int_pretty1 a, Mkspect_evercddl_int_pretty1 b -> rel_evercddl_nint a b
+   | _ -> pure False)) =
+  ()
+
+ghost fn rw_r #a #b (h: squash (a == b)) requires a ensures b { rewrite a as b }
+ghost fn rw_l #a #b (h: squash (a == b)) requires b ensures a { rewrite b as a }
+
+let i32_lt_iff a b : squash (Int32.lt a b <==> Int32.v a < Int32.v b) = ()
+
+fn mk_int (i: Int32.t)
+  returns j: evercddl_int_pretty
+  ensures rel_evercddl_int j (specint_of_i32 i)
+{
+  if Int32.lt i 0l {
+    i32_lt_iff i 0l; assert pure (Int32.v i < Int32.v 0l);
+    let k = Int32.sub (-1l) i;
+    let j = i32_to_u64_safe k;
+    Math.Lemmas.pow2_lt_compat 64 31;
+    rw_l (rel_evercddl_nint_eq (Mkevercddl_nint_pretty0 j) (specnint_of_int (Int32.v i)));
+    rw_l (rel_evercddl_int_eq (Mkevercddl_int_pretty1 (Mkevercddl_nint_pretty0 j)) (Mkspect_evercddl_int_pretty1 (specnint_of_int (Int32.v i))));
+    rewrite each Mkspect_evercddl_int_pretty1 (specnint_of_int (Int32.v i)) as specint_of_i32 i;
+    Mkevercddl_int_pretty1 (Mkevercddl_nint_pretty0 j)
+  } else {
+    let j = i32_to_u64_safe i;
+    rw_l (rel_evercddl_uint_eq (Mkevercddl_uint_pretty0 j) (specuint_of_int (UInt64.v j)));
+    rw_l (rel_evercddl_int_eq (Mkevercddl_int_pretty0 (Mkevercddl_uint_pretty0 j)) (Mkspect_evercddl_int_pretty0 (specuint_of_int (UInt64.v j))));
+    rewrite each Mkspect_evercddl_int_pretty0 (specuint_of_int (UInt64.v j)) as specint_of_i32 i;
+    Mkevercddl_int_pretty0 (Mkevercddl_uint_pretty0 j)
+  }
+}
+
+let rel_sig_structure_eq (a: evercddl_Sig_structure_pretty) (b: spect_evercddl_Sig_structure_pretty) :
+  squash (rel_evercddl_Sig_structure a b == (match a, b with
+    | Mkevercddl_Sig_structure_pretty0 context body_protected rest,
+      Mkspect_evercddl_Sig_structure_pretty0 vcontext vbody_protected vrest ->
+        rel_either rel_unit rel_unit context vcontext **
+        (rel_evercddl_empty_or_serialized_map body_protected vbody_protected **
+          (match rest, vrest with
+            | Inr (aad, payload), Inr (vaad, vpayload) ->
+              rel_evercddl_bstr aad vaad ** rel_evercddl_bstr payload vpayload
+            | Inl (sign_protected, (aad, payload)), Inl (vsign_protected, (vaad, vpayload)) ->
+              rel_evercddl_empty_or_serialized_map sign_protected vsign_protected **
+                (rel_evercddl_bstr aad vaad ** rel_evercddl_bstr payload vpayload)
+            | _ -> pure False)))) =
+  ()
+
+inline_for_extraction noextract
+let signature1: either unit unit = Inr ()
+
+let mk_sig_structure_spec
+    (phdr: spect_evercddl_empty_or_serialized_map_pretty)
+    (aad payload: spect_evercddl_bstr_pretty)
+    : GTot spect_evercddl_Sig_structure_pretty =
+  Mkspect_evercddl_Sig_structure_pretty0 signature1 phdr (Inr (aad, payload))
+
+ghost fn norm_r p s
+  requires p
+  ensures norm s p
+{
+  norm_spec s p;
+  rewrite p as norm s p
+}
+
+let unfold_plus p lids =
+  norm_r p [delta_only lids; iota; primops]
+
+inline_for_extraction noextract
+fn mk_sig_structure phdr aad payload
+  (#vphdr: erased _)
+  (#vaad: erased _)
+  (#vpayload: erased _)
+  requires rel_evercddl_empty_or_serialized_map phdr vphdr
+  requires rel_evercddl_bstr aad vaad
+  requires rel_evercddl_bstr payload vpayload
+  returns r: evercddl_Sig_structure_pretty
+  ensures borrows (rel_evercddl_Sig_structure r (mk_sig_structure_spec vphdr vaad vpayload))
+    (rel_evercddl_empty_or_serialized_map phdr vphdr ** rel_evercddl_bstr aad vaad ** rel_evercddl_bstr payload vpayload)
+{
+  rewrite emp as rel_either rel_unit rel_unit signature1 signature1;
+  rw_l (rel_sig_structure_eq (Mkevercddl_Sig_structure_pretty0 signature1 phdr (Inr (aad, payload)))
+    (Mkspect_evercddl_Sig_structure_pretty0 signature1 vphdr (Inr (reveal vaad, reveal vpayload))));
+  with res vres. assert rel_evercddl_Sig_structure res vres;
+  rewrite each vres as mk_sig_structure_spec vphdr vaad vpayload;
+
+  ghost fn aux ()
+    requires emp ** rel_evercddl_Sig_structure res (mk_sig_structure_spec vphdr vaad vpayload)
+    ensures rel_evercddl_empty_or_serialized_map phdr vphdr ** rel_evercddl_bstr aad vaad ** rel_evercddl_bstr payload vpayload
+  {
+    unfold_plus (rel_evercddl_Sig_structure _ _) [`%mk_sig_structure_spec];
+    rw_r (rel_sig_structure_eq _ _);
+    rewrite rel_either rel_unit rel_unit signature1 signature1 as emp;
+  };
+  intro_trade _ _ _ aux;
+
+  res
+}
+
+let ser_to #t #st (s: CDDL.Spec.Base.spec t st true) (x: st) y =
+  s.serializable x /\ Seq.equal y (CBOR.Spec.API.Format.cbor_det_serialize (s.serializer x))
+
+let ser_to_inj #t #st s x y y' :
+    Lemma (requires ser_to #t #st s x y /\ ser_to s x y') (ensures y == y')
+      [SMTPat (ser_to s x y); SMTPat (ser_to s x y')] =
+  ()
+
+let to_be_signed_spec
+    (phdr: spect_evercddl_empty_or_serialized_map_pretty)
+    (aad payload: spect_evercddl_bstr_pretty)
+    (tbs: Seq.seq UInt8.t)
+    : prop =
+  ser_to bundle_Sig_structure''.b_spec (mk_sig_structure_spec phdr aad payload) tbs
+
+inline_for_extraction noextract
+let sz_to_u32_safe (i: SizeT.t { SizeT.v i < pow2 32 }) : j:UInt32.t { UInt32.v j == SizeT.v i } =
+  Math.Lemmas.small_mod (SizeT.v i) (pow2 32);
+  SizeT.sizet_to_uint32 i
+
+open CommonAbort { abort }
+
+fn create_sig privkey phdr aad payload (sigbuf: S.slice UInt8.t)
+    (#vphdr: erased _) (#vaad: erased _) (#vpayload: erased _) (#pprivkey: erased _)
+    (#vprivkey: erased (Seq.seq UInt8.t) { Seq.length vprivkey == 32 })
+  requires S.pts_to privkey #pprivkey vprivkey
+  requires rel_evercddl_empty_or_serialized_map phdr vphdr
+  requires rel_evercddl_bstr aad vaad
+  requires rel_evercddl_bstr payload vpayload
+  requires exists* vsigbuf. pts_to sigbuf vsigbuf ** pure (Seq.length vsigbuf == 64)
+  ensures S.pts_to privkey #pprivkey vprivkey
+  ensures rel_evercddl_empty_or_serialized_map phdr vphdr
+  ensures rel_evercddl_bstr aad vaad
+  ensures rel_evercddl_bstr payload vpayload
+  ensures exists* tbs.
+    S.pts_to sigbuf (spec_ed25519_sign vprivkey tbs) **
+    pure (to_be_signed_spec vphdr vaad vpayload tbs)
+{
+  let sz = 1024sz;
+  assert pure (SizeT.v sz <= 1024);
+  let arr = V.alloc 0uy sz;
+  Seq.lemma_create_len (SizeT.v sz) 0uy; //?!?
+  V.to_array_pts_to arr;
+  let outbuf = S.from_array (V.vec_to_array arr) sz;
+  S.pts_to_len outbuf;
+  assert pure (S.len outbuf == sz);
+  let sig_struct = mk_sig_structure phdr aad payload;
+  let written = serialize_Sig_structure' sig_struct outbuf;
+  S.pts_to_len outbuf;
+  assert pure (SizeT.v written <= SizeT.v sz);
+  assert pure (SizeT.v written <= 1024);
+  assert_norm (1024 < pow2 32);
+  elim_trade _ _;
+  if (written = 0sz) {
+    abort ();
+    with vsigbuf. rewrite S.pts_to sigbuf vsigbuf as S.pts_to sigbuf (spec_ed25519_sign vprivkey vsigbuf);
+    with voutbuf. rewrite S.pts_to outbuf voutbuf ** S.is_from_array (V.vec_to_array arr) outbuf as emp;
+  } else {
+    let tbs = Pulse.Lib.Slice.Util.subslice_trade outbuf 0sz written;
+    with vtbs. assert S.pts_to tbs vtbs ** pure (to_be_signed_spec vphdr vaad vpayload vtbs);
+    S.pts_to_len tbs;
+    sign sigbuf privkey tbs;
+    elim_trade _ _;
+    S.to_array outbuf;
+    V.to_vec_pts_to arr;
+    V.free arr;
+  }
+}
+
+let rel_inl_map =
+  (CDDL.Pulse.Types.rel_slice_of_table (CDDL.Pulse.Bundle.Base.mk_eq_test_bij
+                    COSE.Format.spect_aux_env25_type_2_pretty_right
+                    COSE.Format.spect_aux_env25_type_2_pretty_left
+                    COSE.Format.spect_aux_env25_type_2_pretty_left_right
+                    COSE.Format.spect_aux_env25_type_2_pretty_right_left
+                    (CDDL.Pulse.Bundle.Base.mk_eq_test_bij COSE.Format.spect_evercddl_label_pretty_right
+                        COSE.Format.spect_evercddl_label_pretty_left
+                        COSE.Format.spect_evercddl_label_pretty_left_right
+                        COSE.Format.spect_evercddl_label_pretty_right_left
+                        (CDDL.Spec.EqTest.either_eq (CDDL.Pulse.Bundle.Base.mk_eq_test_bij COSE.Format.spect_evercddl_int_pretty_right
+                                COSE.Format.spect_evercddl_int_pretty_left
+                                COSE.Format.spect_evercddl_int_pretty_left_right
+                                COSE.Format.spect_evercddl_int_pretty_right_left
+                                (CDDL.Spec.EqTest.either_eq (CDDL.Pulse.Bundle.Base.mk_eq_test_bij COSE.Format.spect_evercddl_uint_pretty_right
+                                        COSE.Format.spect_evercddl_uint_pretty_left
+                                        COSE.Format.spect_evercddl_uint_pretty_left_right
+                                        COSE.Format.spect_evercddl_uint_pretty_right_left
+                                        (CDDL.Spec.EqTest.eqtype_eq FStar.UInt64.t))
+                                    (CDDL.Pulse.Bundle.Base.mk_eq_test_bij COSE.Format.spect_evercddl_nint_pretty_right
+                                        COSE.Format.spect_evercddl_nint_pretty_left
+                                        COSE.Format.spect_evercddl_nint_pretty_left_right
+                                        COSE.Format.spect_evercddl_nint_pretty_right_left
+                                        (CDDL.Spec.EqTest.eqtype_eq FStar.UInt64.t))))
+                            (CDDL.Pulse.Bundle.Base.mk_eq_test_bij COSE.Format.spect_evercddl_tstr_pretty_right
+                                COSE.Format.spect_evercddl_tstr_pretty_left
+                                COSE.Format.spect_evercddl_tstr_pretty_left_right
+                                COSE.Format.spect_evercddl_tstr_pretty_right_left
+                                (CDDL.Spec.EqTest.eqtype_eq (FStar.Seq.Base.seq FStar.UInt8.t))))))
+                COSE.Format.rel_aux_env25_type_2
+                COSE.Format.rel_aux_env25_type_4)
+
+let dummy_map_val () : aux_env25_type_2_pretty & aux_env25_type_4_pretty =
+  Mkaux_env25_type_2_pretty0 (Mkevercddl_label_pretty0
+    (Mkevercddl_int_pretty0 (Mkevercddl_uint_pretty0 0uL))),
+  Mkaux_env25_type_4_pretty0 (Mkevercddl_values_pretty0 (Mkevercddl_any_pretty0
+    { c = CBOR.Pulse.API.Det.Rust.dummy_cbor_det_t (); p = 0.5R }))
+
+let assert_norm' (p: prop) : Pure (squash p) (requires normalize p) (ensures fun _ -> True) = ()
+
+let rel_inl_map_eq (x: slice (aux_env25_type_2_pretty & aux_env25_type_4_pretty)) y = assert_norm' (rel_inl_map x y == 
+  (exists* l .
+    (exists* s . pts_to x.s #x.p s ** Pulse.Lib.SeqMatch.seq_list_match s l (rel_pair rel_aux_env25_type_2 rel_aux_env25_type_4) ** pure (false == false)) **
+      pure (y == map_of_list_pair ((CDDL.Pulse.Bundle.Base.mk_eq_test_bij
+                    COSE.Format.spect_aux_env25_type_2_pretty_right
+                    COSE.Format.spect_aux_env25_type_2_pretty_left
+                    COSE.Format.spect_aux_env25_type_2_pretty_left_right
+                    COSE.Format.spect_aux_env25_type_2_pretty_right_left
+                    (CDDL.Pulse.Bundle.Base.mk_eq_test_bij COSE.Format.spect_evercddl_label_pretty_right
+                        COSE.Format.spect_evercddl_label_pretty_left
+                        COSE.Format.spect_evercddl_label_pretty_left_right
+                        COSE.Format.spect_evercddl_label_pretty_right_left
+                        (CDDL.Spec.EqTest.either_eq (CDDL.Pulse.Bundle.Base.mk_eq_test_bij COSE.Format.spect_evercddl_int_pretty_right
+                                COSE.Format.spect_evercddl_int_pretty_left
+                                COSE.Format.spect_evercddl_int_pretty_left_right
+                                COSE.Format.spect_evercddl_int_pretty_right_left
+                                (CDDL.Spec.EqTest.either_eq (CDDL.Pulse.Bundle.Base.mk_eq_test_bij COSE.Format.spect_evercddl_uint_pretty_right
+                                        COSE.Format.spect_evercddl_uint_pretty_left
+                                        COSE.Format.spect_evercddl_uint_pretty_left_right
+                                        COSE.Format.spect_evercddl_uint_pretty_right_left
+                                        (CDDL.Spec.EqTest.eqtype_eq FStar.UInt64.t))
+                                    (CDDL.Pulse.Bundle.Base.mk_eq_test_bij COSE.Format.spect_evercddl_nint_pretty_right
+                                        COSE.Format.spect_evercddl_nint_pretty_left
+                                        COSE.Format.spect_evercddl_nint_pretty_left_right
+                                        COSE.Format.spect_evercddl_nint_pretty_right_left
+                                        (CDDL.Spec.EqTest.eqtype_eq FStar.UInt64.t))))
+                            (CDDL.Pulse.Bundle.Base.mk_eq_test_bij COSE.Format.spect_evercddl_tstr_pretty_right
+                                COSE.Format.spect_evercddl_tstr_pretty_left
+                                COSE.Format.spect_evercddl_tstr_pretty_left_right
+                                COSE.Format.spect_evercddl_tstr_pretty_right_left
+                                (CDDL.Spec.EqTest.eqtype_eq (FStar.Seq.Base.seq FStar.UInt8.t))))))
+      ) l)))
+
+let sign1_phdrs_spec (alg: Int32.t) =
+  Mkspect_evercddl_empty_or_serialized_map_pretty0
+    (Mkspect_evercddl_header_map_pretty0
+      (Some (Inl (specint_of_i32 alg)))
+      None None None (Inr (Inr (None, None)))
+      (CDDL.Spec.Map.empty _ _))
+
+let rel_map_sign1_phdrs_eq (alg: Int32.t) alg' s =
+  assert_norm' (rel_evercddl_empty_or_serialized_map (Mkevercddl_empty_or_serialized_map_pretty0
+    (Mkevercddl_header_map_pretty0 (Some (Inl alg')) None None None (Inr (Inr (None, None)))
+      (Inl s)))
+    (sign1_phdrs_spec alg) ==
+    (((((rel_evercddl_int alg' (specint_of_i32 alg) **
+      emp) ** emp) ** emp) ** (emp ** emp)) **
+      rel_inl_map s (CDDL.Spec.Map.empty _ _)))
+
+inline_for_extraction
+fn mk_phdrs (alg: Int32.t) (rest: A.larray (aux_env25_type_2_pretty & aux_env25_type_4_pretty) 0)
+    #prest (#vrest: erased _)
+  requires pts_to rest #prest vrest
+  returns res: evercddl_empty_or_serialized_map_pretty
+  ensures borrows (rel_evercddl_empty_or_serialized_map res (sign1_phdrs_spec alg))
+    (pts_to rest #prest vrest)
+{
+  let alg' = mk_int alg;
+  A.pts_to_len rest;
+  let rest2 = S.from_array rest 0sz;
+  Pulse.Lib.SeqMatch.seq_list_match_nil_intro (Seq.Base.create 0 (dummy_map_val ())) []
+      (rel_pair rel_aux_env25_type_2 rel_aux_env25_type_4);
+  assert pure (Seq.Base.create 0 (dummy_map_val ()) `Seq.equal` vrest);
+  rw_l (rel_inl_map_eq {s = rest2; p=prest} (CDDL.Spec.Map.empty _ _));
+  rw_l (rel_map_sign1_phdrs_eq alg alg' _);
+  with res. assert rel_evercddl_empty_or_serialized_map res (sign1_phdrs_spec alg);
+  ghost fn aux ()
+    requires S.is_from_array rest rest2 ** rel_evercddl_empty_or_serialized_map res (sign1_phdrs_spec alg)
+    ensures pts_to rest #prest vrest
+  {
+    rw_r (rel_map_sign1_phdrs_eq alg alg' _);
+    rw_r (rel_inl_map_eq {s = rest2; p=prest} (CDDL.Spec.Map.empty _ _));
+    S.to_array rest2;
+    A.pts_to_len rest;
+    with vrest'. assert pts_to rest #prest vrest';
+    assert pure (Seq.equal vrest' vrest);
+    drop_ (
+      Pulse.Lib.SeqMatch.seq_list_match _ _ (rel_pair rel_aux_env25_type_2 rel_aux_env25_type_4) **
+      rel_evercddl_int alg' (specint_of_i32 alg)
+    );
+  };
+  intro_trade _ _ _ aux;
+  res
+}
+
+let sign1_emphdrs_spec () : GTot _ =
+    (Mkspect_evercddl_header_map_pretty0
+      None None None None (Inr (Inr (None, None)))
+      (CDDL.Spec.Map.empty _ _))
+
+let rel_map_sign1_emphdrs_eq s =
+  assert_norm' (rel_evercddl_header_map (
+    (Mkevercddl_header_map_pretty0 None None None None (Inr (Inr (None, None)))
+      (Inl s)))
+    (sign1_emphdrs_spec ()) ==
+    (((((emp ** emp) ** emp) ** emp) ** (emp ** emp)) **
+      rel_inl_map s (CDDL.Spec.Map.empty _ _)))
+
+inline_for_extraction noextract
+fn mk_emphdrs (rest: A.larray (aux_env25_type_2_pretty & aux_env25_type_4_pretty) 0)
+    #prest (#vrest: erased _)
+  requires pts_to rest #prest vrest
+  returns res: evercddl_header_map_pretty
+  ensures borrows (rel_evercddl_header_map res (sign1_emphdrs_spec ())) (pts_to rest #prest vrest)
+{
+  A.pts_to_len rest;
+  assert pure (Seq.equal vrest (Seq.create 0 (dummy_map_val ())));
+  let rest2 = S.from_array rest 0sz;
+  Pulse.Lib.SeqMatch.seq_list_match_nil_intro (Seq.Base.create 0 (dummy_map_val ())) []
+      (rel_pair rel_aux_env25_type_2 rel_aux_env25_type_4);
+  rw_l (rel_inl_map_eq {s = rest2; p=prest} (CDDL.Spec.Map.empty _ _));
+  rw_l (rel_map_sign1_emphdrs_eq _);
+  with res. assert rel_evercddl_header_map res (sign1_emphdrs_spec ());
+
+  ghost fn aux ()
+    requires S.is_from_array rest rest2 ** rel_evercddl_header_map res (sign1_emphdrs_spec ())
+    ensures pts_to rest #prest vrest
+  {
+    rw_r (rel_map_sign1_emphdrs_eq _);
+    rw_r (rel_inl_map_eq {s = rest2; p=prest} (CDDL.Spec.Map.empty _ _));
+    S.to_array rest2;
+    A.pts_to_len rest;
+    with vrest'. assert pts_to rest #prest vrest';
+    assert pure (Seq.equal vrest' vrest);
+    drop_ (
+      Pulse.Lib.SeqMatch.seq_list_match _ _ (rel_pair rel_aux_env25_type_2 rel_aux_env25_type_4)
+    );
+  };
+  intro_trade _ _ _ aux;
+
+  res
+}
+
+let sign1_tagged_spec (alg: Int32.t) uhdr payload sig =
+  Mkspect_evercddl_COSE_Sign1_Tagged_pretty0 (Mkspect_evercddl_COSE_Sign1_pretty0
+    (sign1_phdrs_spec alg) uhdr (Inl payload) sig)
+
+let rel_sign1_tagged_eq1 phdr uhdr payload sig vphdr vuhdr vpayload vsig =
+  assert_norm' (rel_evercddl_COSE_Sign1_Tagged
+      (Mkevercddl_COSE_Sign1_Tagged_pretty0
+        (Mkevercddl_COSE_Sign1_pretty0 phdr uhdr (Inl payload) sig))
+      (Mkspect_evercddl_COSE_Sign1_Tagged_pretty0 (Mkspect_evercddl_COSE_Sign1_pretty0
+        vphdr vuhdr (Inl vpayload) vsig)) ==
+  (rel_evercddl_empty_or_serialized_map phdr vphdr **
+    rel_evercddl_header_map uhdr vuhdr) **
+    (rel_evercddl_bstr payload vpayload ** rel_evercddl_bstr sig vsig))
+
+let rel_bstr_eq (x: evercddl_bstr_pretty) (y: spect_evercddl_bstr_pretty) =
+  assert_norm' (rel_evercddl_bstr x y ==
+    (match x, y with
+    | Mkevercddl_bstr_pretty0 { s; p }, Mkspect_evercddl_bstr_pretty0 y ->
+      pts_to s #p y ** pure (false == false))
+    )
+
+ghost fn rw_r_wt #a #b (h: squash (a == b)) requires a ensures b ** trade b a { rewrite_with_trade a b }
+ghost fn rw_l_wt #a #b (h: squash (a == b)) requires b ensures a ** trade a b { rewrite_with_trade b a }
+
+let sign1_spec
+    privkey
+    (uhdr: spect_evercddl_header_map_pretty)
+    (aad payload: spect_evercddl_bstr_pretty)
+    (msg: Seq.seq UInt8.t)
+    : prop =
+  let phdr = sign1_phdrs_spec (-8l) in
+  exists tbs. to_be_signed_spec phdr aad payload tbs /\
+  ser_to bundle_COSE_Sign1_Tagged''.b_spec
+    (Mkspect_evercddl_COSE_Sign1_Tagged_pretty0 (Mkspect_evercddl_COSE_Sign1_pretty0
+        phdr uhdr (Inl payload) { _x0 = spec_ed25519_sign privkey tbs }))
+    msg
+
+ghost fn trade_exists (#t: Type0) (p: t->slprop) x
+  ensures trade (p x) (exists* y. p y)
+{
+  ghost fn aux ()
+    requires emp ** p x
+    ensures exists* y. p y
+  { () };
+  intro_trade _ _ _ aux;
+}
+
+inline_for_extraction // Karamel's lifetime support is massively lacking
+fn sign1 privkey uhdr aad payload (outbuf: S.slice UInt8.t)
+    #pprivkey (#vprivkey: erased (Seq.seq UInt8.t) { Seq.length vprivkey == 32 })
+    (#vuhdr: erased _) (#vaad: erased _) (#vpayload: erased _)
+  requires S.pts_to privkey #pprivkey vprivkey
+  requires rel_evercddl_header_map uhdr vuhdr
+  requires rel_evercddl_bstr aad vaad
+  requires rel_evercddl_bstr payload vpayload
+  requires exists* voutbuf. pts_to outbuf voutbuf
+
+  returns out: S.slice UInt8.t
+  ensures S.pts_to privkey #pprivkey vprivkey
+  ensures rel_evercddl_header_map uhdr vuhdr
+  ensures rel_evercddl_bstr aad vaad
+  ensures rel_evercddl_bstr payload vpayload
+  ensures exists* msg.
+    borrows (S.pts_to out msg) (exists* voutbuf. pts_to outbuf voutbuf) **
+    pure (sign1_spec vprivkey vuhdr vaad vpayload msg)
+{
+  let alg: Int32.t = -8l;
+  let mut phdrauxbuf = [| dummy_map_val (); 0sz |];
+  let phdr = mk_phdrs alg phdrauxbuf;
+  let mut sigbuf = [| 0uy; 64sz |];
+  Seq.lemma_create_len (SizeT.v 64sz) 0uy; //?!?
+  let sigbuf2 = S.from_array sigbuf 64sz;
+  create_sig privkey phdr aad payload sigbuf2;
+  // S.to_array sigbuf2 #_ #(spec_ed25519_sign vprivkey _);
+  with tbs. assert S.pts_to sigbuf2 (spec_ed25519_sign vprivkey tbs);
+  // let sigbuf3 = S.from_array sigbuf 64sz;
+  with sigbuf4. assert pure ((sigbuf4 <: evercddl_bstr_pretty) == { _x0 = { p = 1.0R; s = sigbuf2 } });
+  rw_l_wt (rel_bstr_eq sigbuf4 { _x0 = spec_ed25519_sign vprivkey tbs });
+  rw_l_wt (rel_sign1_tagged_eq1 phdr _ payload sigbuf4 (sign1_phdrs_spec alg) _ vpayload _);
+  let outbuf_sz = serialize_COSE_Sign1_Tagged' _ outbuf;
+  elim_trade (rel_evercddl_COSE_Sign1_Tagged _ _) _;
+  elim_trade (rel_evercddl_bstr sigbuf4 { _x0 = spec_ed25519_sign vprivkey tbs }) _;
+  S.to_array sigbuf2;
+  elim_trade _ _;
+  with voutbuf. assert S.pts_to outbuf voutbuf;
+  trade_exists (S.pts_to outbuf) voutbuf;
+  if (outbuf_sz = 0sz) {
+    abort ();
+    assert S.pts_to outbuf (spec_ed25519_sign vprivkey tbs);
+    outbuf
+  } else {
+    let out = Pulse.Lib.Slice.Util.subslice_trade outbuf 0sz outbuf_sz;
+    trade_compose _ (S.pts_to outbuf _) _;
+    out;
+  }
+}
+
+fn sign1_simple privkey payload (outbuf: S.slice UInt8.t)
+    #pprivkey (#vprivkey: erased (Seq.seq UInt8.t) { Seq.length vprivkey == 32 })
+    (#vpayload: erased _)
+    (#voutbuf: erased _)
+  requires S.pts_to privkey #pprivkey vprivkey
+  requires rel_evercddl_bstr payload vpayload
+  requires pts_to outbuf voutbuf
+
+  returns out: S.slice UInt8.t
+  ensures S.pts_to privkey #pprivkey vprivkey
+  ensures rel_evercddl_bstr payload vpayload
+  ensures exists* msg.
+    borrows (S.pts_to out msg) (exists* voutbuf. pts_to outbuf voutbuf) **
+    pure (sign1_spec vprivkey (sign1_emphdrs_spec ()) { _x0 = Seq.create 0 0uy } vpayload msg)
+{
+  let mut uhdrauxbuf = [| dummy_map_val (); 0sz |];
+  let uhdr = mk_emphdrs uhdrauxbuf;
+  let mut aadbuf = [| 0uy; 0sz |];
+  let aadslice = S.from_array aadbuf 0sz;
+  with aad. assert pure ((aad <: evercddl_bstr_pretty) == Mkevercddl_bstr_pretty0 { s = aadslice; p = 1.0R });
+  rw_l (rel_bstr_eq aad (Mkspect_evercddl_bstr_pretty0 _));
+  let res = sign1 privkey uhdr aad payload outbuf;
+  with msg. assert pts_to res msg;
+  rw_r (rel_bstr_eq aad (Mkspect_evercddl_bstr_pretty0 _));
+  S.to_array aadslice;
+  elim_trade _ (A.pts_to uhdrauxbuf _);
+  res
+}
+
+fn verify_sig pubkey phdr aad payload (sigbuf: S.slice UInt8.t)
+    (#vphdr: erased _) (#vaad: erased _) (#vpayload: erased _) (#ppubkey: erased _)
+    #psigbuf (#vsigbuf: erased (Seq.seq UInt8.t) { Seq.length vsigbuf == 64 })
+    (#vpubkey: erased (Seq.seq UInt8.t) { Seq.length vpubkey == 32 })
+  requires S.pts_to pubkey #ppubkey vpubkey
+  requires rel_evercddl_empty_or_serialized_map phdr vphdr
+  requires rel_evercddl_bstr aad vaad
+  requires rel_evercddl_bstr payload vpayload
+  requires pts_to sigbuf #psigbuf vsigbuf
+  returns success: bool
+  ensures S.pts_to pubkey #ppubkey vpubkey
+  ensures rel_evercddl_empty_or_serialized_map phdr vphdr
+  ensures rel_evercddl_bstr aad vaad
+  ensures rel_evercddl_bstr payload vpayload
+  ensures pts_to sigbuf #psigbuf vsigbuf
+  ensures pure (success <==> (exists tbs. to_be_signed_spec vphdr vaad vpayload tbs /\ spec_ed25519_verify vpubkey tbs vsigbuf))
+{
+  let sz = 1024sz;
+  assert pure (SizeT.v sz <= 1024);
+  let arr = V.alloc 0uy sz;
+  Seq.lemma_create_len (SizeT.v sz) 0uy; //?!?
+  V.to_array_pts_to arr;
+  let outbuf = S.from_array (V.vec_to_array arr) sz;
+  S.pts_to_len outbuf;
+  assert pure (S.len outbuf == sz);
+  let sig_struct = mk_sig_structure phdr aad payload;
+  let written = serialize_Sig_structure' sig_struct outbuf;
+  S.pts_to_len outbuf;
+  assert pure (SizeT.v written <= SizeT.v sz);
+  assert pure (SizeT.v written <= 1024);
+  assert_norm (1024 < pow2 32);
+  elim_trade _ _;
+  if (written = 0sz) {
+    abort ();
+    with w. rewrite S.pts_to outbuf w ** S.is_from_array (V.vec_to_array arr) outbuf as emp;
+    false
+  } else {
+    let tbs = Pulse.Lib.Slice.Util.subslice_trade outbuf 0sz written;
+    with vtbs. assert S.pts_to tbs vtbs ** pure (to_be_signed_spec vphdr vaad vpayload vtbs);
+    S.pts_to_len tbs;
+    let success = verify pubkey tbs sigbuf;
+    elim_trade _ _;
+    S.to_array outbuf;
+    V.to_vec_pts_to arr;
+    V.free arr;
+    success
+  }
+}
+
+let rel_sign1_tagged_eq (a: evercddl_COSE_Sign1_Tagged_pretty) (b: spect_evercddl_COSE_Sign1_Tagged_pretty) =
+  assert_norm' (rel_evercddl_COSE_Sign1_Tagged a b ==
+    ((COSE.Format.rel_evercddl_empty_or_serialized_map a._x0.protected b._x0._x0 **
+            COSE.Format.rel_evercddl_header_map a._x0.unprotected b._x0._x1) **
+        ((CDDL.Pulse.Types.rel_either COSE.Format.rel_evercddl_bstr
+                COSE.Format.rel_evercddl_nil a._x0.payload b._x0._x2) **
+            COSE.Format.rel_evercddl_bstr a._x0.signature b._x0._x3))
+    )
+
+let rel_bstr_eq' (x: evercddl_bstr_pretty) (y: spect_evercddl_bstr_pretty) =
+  assert_norm' (rel_evercddl_bstr x y ==
+      pts_to x._x0.s #x._x0.p y._x0 ** pure (false == false))
+
+inline_for_extraction noextract
+let sixty_four: v: SizeT.t { SizeT.v v == 64 } = 64sz
+
+inline_for_extraction noextract
+fn verify1_core pubkey aad (msg: evercddl_COSE_Sign1_Tagged_pretty { Inl? msg._x0.payload })
+    #ppubkey (#vpubkey: erased (Seq.seq UInt8.t) { Seq.length vpubkey == 32 })
+    (#vaad: erased _) (#vmsg: erased spect_evercddl_COSE_Sign1_Tagged_pretty { Inl? (reveal vmsg)._x0._x2 })
+  requires S.pts_to pubkey #ppubkey vpubkey
+  requires rel_evercddl_COSE_Sign1_Tagged msg vmsg
+  requires rel_evercddl_bstr aad vaad
+
+  returns success: bool
+  ensures S.pts_to pubkey #ppubkey vpubkey
+  ensures rel_evercddl_COSE_Sign1_Tagged msg vmsg
+  ensures rel_evercddl_bstr aad vaad
+  ensures pure (success <==>
+      (let sig = (reveal vmsg)._x0._x3._x0 in
+        Seq.length sig == 64 /\
+        exists (tbs: Seq.seq UInt8.t{Seq.length tbs <= max_size_t}).
+        to_be_signed_spec (reveal vmsg)._x0._x0 vaad (Inl?.v (reveal vmsg)._x0._x2) tbs /\
+        spec_ed25519_verify vpubkey tbs sig))
+{
+  rw_r_wt (rel_sign1_tagged_eq _ _);
+  rw_r_wt (rel_bstr_eq' msg._x0.signature _);
+  rewrite_with_trade
+    (rel_either rel_evercddl_bstr rel_evercddl_nil msg._x0.payload (reveal vmsg)._x0._x2)
+    (rel_evercddl_bstr (Inl?.v msg._x0.payload) (Inl?.v (reveal vmsg)._x0._x2));
+  let sig = msg._x0.signature._x0.s;
+  rewrite each msg._x0.signature._x0.s as sig;
+  S.pts_to_len sig;
+  with vsig. assert S.pts_to sig #msg._x0.signature._x0.p vsig;
+  if (S.len sig = sixty_four) {
+    assert pure (S.len sig == sixty_four);
+    assert pure (SizeT.v (S.len sig) == 64);
+    assert pure (Seq.length vsig == 64);
+    let success = verify_sig pubkey msg._x0.protected aad (Inl?.v msg._x0.payload) sig;
+    elim_trade _ (rel_evercddl_bstr msg._x0.signature _);
+    elim_trade _ (rel_either rel_evercddl_bstr rel_evercddl_nil msg._x0.payload (reveal vmsg)._x0._x2);
+    elim_trade _ (rel_evercddl_COSE_Sign1_Tagged msg vmsg);
+    success
+  } else {
+    elim_trade _ (rel_evercddl_bstr msg._x0.signature _);
+    elim_trade _ (rel_either rel_evercddl_bstr rel_evercddl_nil msg._x0.payload (reveal vmsg)._x0._x2);
+    elim_trade _ (rel_evercddl_COSE_Sign1_Tagged msg vmsg);
+    assert pure (Seq.length vsig =!= 64);
+    assert pure ((reveal vmsg)._x0._x3._x0 == vsig);
+    false
+  }
+}
+
+inline_for_extraction noextract
+fn borrow_payload
+    (msg: evercddl_COSE_Sign1_Tagged_pretty { Inl? msg._x0.payload })
+    (#vmsg: erased spect_evercddl_COSE_Sign1_Tagged_pretty { Inl? (reveal vmsg)._x0._x2 })
+  requires rel_evercddl_COSE_Sign1_Tagged msg vmsg
+  returns payload: S.slice UInt8.t
+  ensures
+    borrows (pts_to payload #((Inl?.v msg._x0.payload)._x0.p) (Inl?.v (reveal vmsg)._x0._x2)._x0)
+      (rel_evercddl_COSE_Sign1_Tagged msg vmsg)
+{
+  rw_r (rel_sign1_tagged_eq _ _);
+  rewrite_with_trade
+    (rel_either rel_evercddl_bstr rel_evercddl_nil msg._x0.payload (reveal vmsg)._x0._x2)
+    (rel_evercddl_bstr (Inl?.v msg._x0.payload) (Inl?.v (reveal vmsg)._x0._x2));
+  rw_r (rel_bstr_eq' (Inl?.v msg._x0.payload) _);
+  ghost fn aux ()
+    requires
+      rel_evercddl_bstr msg._x0.signature (reveal vmsg)._x0._x3 **
+      rel_evercddl_empty_or_serialized_map msg._x0.protected (reveal vmsg)._x0._x0 **
+      rel_evercddl_header_map msg._x0.unprotected (reveal vmsg)._x0._x1 **
+      trade (rel_evercddl_bstr (Inl?.v msg._x0.payload) (Inl?.v (reveal vmsg)._x0._x2))
+        (rel_either rel_evercddl_bstr
+            rel_evercddl_nil
+            msg._x0.payload
+            (reveal vmsg)._x0._x2)
+    requires S.pts_to (Inl?.v msg._x0.payload)._x0.s #(Inl?.v msg._x0.payload)._x0.p
+      (Inl?.v (reveal vmsg)._x0._x2)._x0
+    ensures rel_evercddl_COSE_Sign1_Tagged msg vmsg
+  {
+    rw_l (rel_bstr_eq' (Inl?.v msg._x0.payload) _);
+    elim_trade _ _;
+    rw_l (rel_sign1_tagged_eq _ _);
+  };
+  intro_trade _ _ _ aux;
+  (Inl?.v msg._x0.payload)._x0.s
+}
+
+noextract
+let parses_from #t #st (s: CDDL.Spec.Base.spec t st true) (x: st) y : prop =
+  match CBOR.Spec.API.Format.cbor_det_parse y with
+  | Some (c, len) -> len == Seq.length y /\ t c /\ s.parser c == x
+  | None -> False
+
+let good_signature (pubkey: Seq.seq UInt8.t { Seq.length pubkey == 32 })
+    (msg: Seq.seq UInt8.t) (aad: Seq.seq UInt8.t) (payload: Seq.seq UInt8.t) : prop =
+  exists (vmsg: spect_evercddl_COSE_Sign1_Tagged_pretty) tbs.
+  parses_from bundle_COSE_Sign1_Tagged''.b_spec vmsg msg /\
+  vmsg._x0._x2 == Inl (Mkspect_evercddl_bstr_pretty0 payload) /\
+  Seq.length vmsg._x0._x3._x0 == 64 /\
+  to_be_signed_spec vmsg._x0._x0 { _x0 = aad } { _x0 = payload } tbs /\
+  spec_ed25519_verify pubkey tbs vmsg._x0._x3._x0
+
+let int_eq_of_diff_zero (a b: int) : Lemma (requires a - b == 0) (ensures a == b) = ()
+let nat_eq_of_diff_zero (a b: nat) : Lemma (requires a - b == 0) (ensures a == b) =
+  int_eq_of_diff_zero a b
+
+inline_for_extraction // Karamel's lifetime support is massively lacking
+fn verify1 pubkey aad msg
+    #ppubkey (#vpubkey: erased (Seq.seq UInt8.t) { Seq.length vpubkey == 32 })
+    (#vaad: erased _) #pmsg (#vmsg: erased _)
+  requires S.pts_to pubkey #ppubkey vpubkey
+  requires S.pts_to #UInt8.t msg #pmsg vmsg
+  requires rel_evercddl_bstr aad vaad
+
+  returns payload: option (S.slice UInt8.t)
+
+  ensures S.pts_to pubkey #ppubkey vpubkey
+  ensures rel_evercddl_bstr aad vaad
+  ensures
+    (match payload with
+    | Some payload ->
+      exists* ppayload vpayload.
+        borrows (S.pts_to payload #ppayload vpayload) (S.pts_to msg #pmsg vmsg) **
+        pure (good_signature vpubkey vmsg (reveal vaad)._x0 vpayload)
+    | None -> S.pts_to msg #pmsg vmsg)
+{
+  let res = validate_and_parse_COSE_Sign1_Tagged msg;
+  match res {
+    None -> {
+      unfold CDDL.Pulse.Parse.Base.validate_and_parse_post;
+      None
+    }
+    Some res -> {
+      match res {
+        (x, rem) -> {
+          unfold CDDL.Pulse.Parse.Base.validate_and_parse_post;
+          unfold CDDL.Pulse.Parse.Base.validate_and_parse_post_some bundle_COSE_Sign1_Tagged.b_spec.CDDL.Spec.Base.parser
+            rel_evercddl_COSE_Sign1_Tagged msg pmsg vmsg x rem;
+          with y. assert rel_evercddl_COSE_Sign1_Tagged x y;
+          with wr. assert pts_to rem #pmsg wr;
+
+          rw_r_wt (rel_sign1_tagged_eq _ _);
+          rel_either_cases _ _ _ _;
+          elim_trade _ (rel_evercddl_COSE_Sign1_Tagged _ _);
+
+          if (S.len rem = 0sz && Inl? x._x0.payload) {
+            let len = hide (Some?.v (CBOR.Spec.API.Format.cbor_det_parse vmsg))._2;
+            S.pts_to_len rem;
+            assert pure (Seq.length wr == 0);
+            Seq.lemma_len_slice vmsg len (Seq.length vmsg);
+            nat_eq_of_diff_zero (Seq.length vmsg) len;
+            assert pure (parses_from bundle_COSE_Sign1_Tagged''.b_spec y vmsg);
+            let success = verify1_core pubkey aad x;
+            if (success) {
+              let payload = borrow_payload x;
+              elim_hyp_r _ _ _;
+              trade_compose _ (rel_evercddl_COSE_Sign1_Tagged _ _) _;
+              Some payload
+            } else {
+              elim_trade _ (S.pts_to msg #pmsg vmsg);
+              None
+            }
+          } else {
+            elim_trade _ (S.pts_to msg #pmsg vmsg);
+            None
+          }
+        }
+      }
+    }
+  }
+}
+
+fn verify1_simple pubkey msg
+    #ppubkey (#vpubkey: erased (Seq.seq UInt8.t) { Seq.length vpubkey == 32 })
+    #pmsg (#vmsg: erased _)
+  requires S.pts_to pubkey #ppubkey vpubkey
+  requires S.pts_to #UInt8.t msg #pmsg vmsg
+
+  returns payload: option (S.slice UInt8.t)
+  ensures S.pts_to pubkey #ppubkey vpubkey
+  ensures
+    (match payload with
+    | Some payload ->
+      exists* ppayload vpayload.
+        borrows (S.pts_to payload #ppayload vpayload) (S.pts_to msg #pmsg vmsg) **
+        pure (good_signature vpubkey vmsg (Seq.create 0 0uy) vpayload)
+    | None -> S.pts_to msg #pmsg vmsg)
+{
+  let mut aadbuf = [| 0uy; 0sz |];
+  let aadslice = S.from_array aadbuf 0sz;
+  with aad. assert pure ((aad <: evercddl_bstr_pretty) == Mkevercddl_bstr_pretty0 { s = aadslice; p = 1.0R });
+  rw_l (rel_bstr_eq aad (Mkspect_evercddl_bstr_pretty0 _));
+  let res = verify1 pubkey aad msg;
+  rw_r (rel_bstr_eq aad (Mkspect_evercddl_bstr_pretty0 _));
+  S.to_array aadslice;
+  res
+}
