src/cose/rust/EverCrypt.Ed25519.fst
@@ -1,0 +1,43 @@
+module EverCrypt.Ed25519
+open Pulse
+#lang-pulse
+
+let spec_ed25519_sign secret msg = Seq.create 64 0uy
+
+fn sign
+    (signature:S.slice U8.t)
+    (#p_private_key: perm)
+    (#v_private_key: Ghost.erased (Seq.seq U8.t) { Seq.length v_private_key == 32 })
+    (private_key:S.slice U8.t)
+    (#p_msg: perm)
+    (#v_msg: Ghost.erased (Seq.seq U8.t) { Seq.length v_msg <= max_size_t })
+    (msg:S.slice U8.t)
+  requires
+    (exists* v_signature . pts_to signature v_signature ** pure (Seq.length v_signature == 64)) **
+    pts_to private_key #p_private_key v_private_key **
+    pts_to msg #p_msg v_msg
+  returns _: squash (Seq.length v_private_key == 32)
+  ensures
+    S.pts_to signature (spec_ed25519_sign v_private_key v_msg) **
+    pts_to private_key #p_private_key v_private_key **
+    pts_to msg #p_msg v_msg
+{
+  S.(signature.(0sz) <- 0uy);
+  admit ()
+}
+
+let spec_ed25519_verify public msg sig = true
+
+fn verify
+    (#p_public_key: perm)
+    (#v_public_key: Ghost.erased (Seq.seq U8.t) { Seq.length v_public_key == 32 })
+    (public_key:S.slice U8.t)
+    (#p_msg: perm)
+    (#v_msg: Ghost.erased (Seq.seq U8.t) { Seq.length v_msg <= max_size_t })
+    (msg:S.slice U8.t)
+    (#p_signature: perm)
+    (#v_signature: Ghost.erased (Seq.seq U8.t) { Seq.length v_signature == 64 })
+    (signature:S.slice U8.t)
+{
+  admit ()
+}
